Attempted simplification; but can't obtain pi in backtranslation

ModelingLanguage.fst
@@ -19,9 +19,10 @@ assume val pt : (m:Type->Type) -> Type0
 
 let ctx : Type = mon:monad -> acts mon -> ct mon.m
 
-let prog : Type = mon:monad -> a:acts mon -> ct mon.m -> pt mon.m
-
 assume val free : monad
+
+let prog : Type = ct free.m -> pt free.m
+
 let stuff = string (* TODO: cheating, to be fixed later *)
 assume val check_get_trace : stuff -> free.m bool
 assume val bind_free : #a:Type -> #b:Type -> free.m a -> (a -> free.m b) -> free.m b
@@ -36,24 +37,37 @@ let wrapped_acts : acts free = {
     bind_free (check_get_trace s) (fun b -> if b then free_acts.read s else free.ret None)
 }
 
-let link (p:prog) (c:ctx) : whole = (p free free_acts (c free wrapped_acts))
+let link (p:prog) (c:ctx) : whole = p (c free wrapped_acts)
 
 (* used to state transparency *)
 (* forall p c pi. link_no_check p c ~> t /\ t \in pi => link p c ~> t *)
-let link_no_check (p:prog) (c:ctx) : whole = (p free free_acts (c free free_acts))
+let link_no_check (p:prog) (c:ctx) : whole = p (c free free_acts)
 
 assume val ictx : Type0
 assume val iwhole : Type0
 let iprog : Type0 = ictx -> iwhole
 (* TODO: this needs to be/include IIO pi arrow; which may bring back reification? in compile_whole? on the argument of compile_whole? *)
 
-assume val backtranslate (mon:monad) : ct mon.m -> ictx
-assume val compile_whole (mon:monad) : iwhole -> pt mon.m
+(* TODO: these will need to be type-classes depending on structure of ct and pt *)
+assume val backtranslate : ct free.m -> ictx
+assume val compile_whole : iwhole -> pt free.m
 
-let compile (p:iprog) : prog = fun mon a c -> compile_whole mon (p (backtranslate mon c))
+let compile (ip:iprog) : prog = fun (c:ct free.m) -> compile_whole (ip (backtranslate c))
+
+(* soundness *)
+(* forall ip c pi. compile ip `link pi` c ~> t => t \in pi *)
 
 
 
+(* Example:
+   ct free.m = alpha -> free.m beta
+   ictx for this = alpha -> IIO beta pi
+*)
+
+assume val alpha : Type0
+assume val beta : Type0
+let bt (pi:...) (f : (alpha -> free.m beta)) (a:alpha) : IIO beta pi =
+  IIO?.reflect (f a) (* TODO: but how do he get that pi holds, if we can get actions that weren't wrapped, as done in link_no_check! *)
 
 (* Possible issue: backtranslation may be difficult if we allow m at arbitrary places,
    while in F* effects are only allowed at the right or arrows;
